

NANYANG TECHNOLOGICAL UNIVERSITY  
SPMS/DIVISION OF MATHEMATICAL SCIENCES

2025/26 Semester 2    MH4110 Partial Differential Equations    Tutorial 2, 29 January

**Problem 1 (Ex. 1 on Page 9).** Solve the first-order equation

$$2u_t + 3u_x = 0$$

subject to the initial condition  $u(0, x) = \sin x$ .

**Solution.** The characteristic curves satisfy

$$3t - 2x = c.$$

The solution is constant along each characteristic curve, so the general solution has the form

$$u(t, x) = f(3t - 2x).$$

Imposing the initial condition at  $t = 0$ , we obtain

$$\sin x = u(0, x) = f(-2x).$$

Letting  $w = -2x$ , we find  $f(w) = \sin(-w/2)$ . Hence,

$$u(t, x) = \sin\left(\frac{-3t + 2x}{2}\right).$$

**Problem 2.** Solve

$$3u_x - 5u_y = 0$$

subject to the condition  $u(0, y) = \cos y$ .

**Solution.** The characteristic curves are given by

$$-5x - 3y = c.$$

Thus, the general solution is

$$u(x, y) = f(-5x - 3y).$$

Applying the condition at  $x = 0$ ,

$$\cos y = u(0, y) = f(-3y),$$

which implies  $f(w) = \cos(-w/3)$ . Therefore,

$$u(x, y) = \cos\left(\frac{5x + 3y}{3}\right).$$

**Problem 3 (Ex. 2 on Page 9)** Solve the equation  $3u_y + u_{xy} = 0$ .

[Solution:] Letting  $v = u_y$ , we can write the equation as a system:

$$u_y = v, \quad v_x + 3v = 0.$$

We first solve the second equation:  $v_x + 3v = 0$ . Treating  $y$  as a parameter, we obtain  $v(x, y) = C(y)e^{-3x}$ . Integrating  $v$ , we obtain the solution:  $u(x, y) = D(y)e^{-3x} + E(x)$ , where we denoted  $D(y) = \int C(y)dy$ . Here,  $D$  and  $E$  are arbitrary functions.

**Problem 4 (Modified from Ex. 9 on Page 10)** Use both the geometric method and the coordinate method to solve the equation

$$u_x + u_y = 1.$$

[Solution:]

- (a) The geometric method. This is an inhomogeneous PDE. Assuming that a particular solution to this PDE takes a form as  $u(x, y) = Ax$ , we can plug it into the PDE and get  $A = 1$ . For the homogeneous PDE  $u_x + u_y = 0$ , its characteristic lines are given by  $x - y = C$ , where  $C$  is an arbitrary constant. So the solution of the homogeneous PDE is  $u(x, y) = f(x - y)$ . Thus, the solution of  $u_x + u_y = 1$  is

$$u(x, y) = x + f(x - y),$$

where  $f$  is an arbitrary function.

- (b) The coordinate method  
Change variables to

$$x' = x + y \quad \text{and} \quad y' = x - y,$$

we have

$$\frac{\partial}{\partial x} = \frac{\partial x'}{\partial x} \frac{\partial}{\partial x'} + \frac{\partial y'}{\partial x} \frac{\partial}{\partial y'} = \frac{\partial}{\partial x'} + \frac{\partial}{\partial y'},$$

and

$$\frac{\partial}{\partial y} = \frac{\partial x'}{\partial y} \frac{\partial}{\partial x'} + \frac{\partial y'}{\partial y} \frac{\partial}{\partial y'} = \frac{\partial}{\partial x'} - \frac{\partial}{\partial y'}.$$

So the PDE is transformed into

$$u_{x'} = \frac{1}{2}.$$

Consider  $y'$  as a parameter, this equation can be viewed as a first-order inhomogeneous ODE with the independent variable  $x'$ . Integrating with respect to  $x'$ , we have

$$u = \frac{x'}{2} + f(y').$$

$f$  is an arbitrary function of a single variable. Change back to the original coordinates, we have the solution

$$u(x, y) = \frac{x + y}{2} + f(x - y).$$

**Problem 5** Solve  $au_x + bu_y = c$  using the coordinate method, where  $a, b, c$  are constants and  $a \neq 0$ .

[Solution:] Change variables to

$$x' = ax + by \quad y' = bx - ay$$

Replace all  $x$  and  $y$  derivatives by  $x'$  and  $y'$  derivatives. By the chain rule,

$$u_x = \frac{\partial u}{\partial x} = \frac{\partial u}{\partial x'} \frac{\partial x'}{\partial x} + \frac{\partial u}{\partial y'} \frac{\partial y'}{\partial x} = au_{x'} + bu_{y'}$$

and

$$u_y = \frac{\partial u}{\partial y} = \frac{\partial u}{\partial x'} \frac{\partial x'}{\partial y} + \frac{\partial u}{\partial y'} \frac{\partial y'}{\partial y} = bu_{x'} - au_{y'}.$$

Hence  $c = au_x + bu_y = a(au_{x'} + bu_{y'}) + b(bu_{x'} - au_{y'}) = (a^2 + b^2)u_{x'}$ . Since  $a^2 + b^2 \neq 0$ , the equation takes the form  $u_{x'} = c/(a^2 + b^2)$  in the new (primed) variables. Thus the solution is  $u = cx'/(a^2 + b^2) + f(y')$ , with  $f$  an arbitrary function. The solution in the original coordinates is  $u = c(ax + by)/(a^2 + b^2) + f(bx - ay)$ .

**Problem 6** Solve the equation  $yu_x + xu_y = 0$  with the condition  $u(0, y) = y$ . In which region of the  $xy$  plane is the solution uniquely determined?

[Solution:] (a) The characteristic curves are given by  $\frac{dy}{dx} = \frac{x}{y}$ . This is a separable ODE. Its solution is  $y^2 = x^2 + C$ , where  $C$  is any given constant. Then, the general solution of the original PDE is  $u(x, y) = f(y^2 - x^2)$ . The auxiliary condition says  $u(0, y) = y$ . Substituting  $x = 0$  into the general solution, we have  $y = f(y^2)$ . We can only determine the explicit form of  $f(y^2)$  as  $f(y^2) = \sqrt{y^2} = y$  when  $y \geq 0$  or  $f(y^2) = -\sqrt{y^2} = y$  when  $y < 0$ . Thus,

$$u(x, y) = \begin{cases} \sqrt{y^2 - x^2}, & \text{if } y^2 \geq x^2 \text{ and } y \geq 0; \\ -\sqrt{y^2 - x^2}, & \text{if } y^2 \geq x^2 \text{ and } y < 0; \\ f(y^2 - x^2), & \text{if } y^2 < x^2. \end{cases}$$

(b) From the above discussion, we know that the solution is uniquely determined when  $y^2 \geq x^2$ .

**Problem 7** Find the general solution of

$$u_x + e^y u_y = 1.$$

[Solution:] We look for the characteristic curve  $y = y(x)$  satisfying

$$\frac{dy}{dx} = \frac{e^y}{1} = e^y \Rightarrow x + e^{-y} = C.$$

Hence, the general solution of the problem is

$$u(x, y) = f(x + e^{-y}).$$

Obviously,  $u(x, y) = x$  is a particular solution. Thus, the solution of the original problem is

$$u(x, y) = f(x + e^{-y}) + x.$$

**Problem 8 (Ex. 6 on Page 10)** Solve the equation

$$\sqrt{1 - x^2} u_x + u_y = 0, \quad u(0, y) = y.$$

[Solution:] We look for the characteristic curve  $y = y(x)$  satisfying

$$\frac{dy}{dx} = \frac{1}{\sqrt{1 - x^2}} \Rightarrow y(x) = \arcsin x + C.$$

Hence, the general solution of the problem is

$$u(x, y) = f(y - \arcsin x).$$

As  $u(0, y) = f(y) = y$ , we have that the solution is  $u(x, y) = y - \arcsin x$ .

**Problem 9** Find the general solution of the equation

$$(a) \quad -2u_x + u_y + 3u = e^{x+y};$$

$$(b) \quad xu_x - yu_y + y^2u = y^2, \quad x, y \neq 0.$$

[Solution:]

(a) Change variables to

$$x' = -2x + y \quad \text{and} \quad y' = x + 2y,$$

we have

$$\frac{\partial}{\partial x} = \frac{\partial x'}{\partial x} \frac{\partial}{\partial x'} + \frac{\partial y'}{\partial x} \frac{\partial}{\partial y'} = -2 \frac{\partial}{\partial x'} + \frac{\partial}{\partial y'},$$

and

$$\frac{\partial}{\partial y} = \frac{\partial x'}{\partial y} \frac{\partial}{\partial x'} + \frac{\partial y'}{\partial y} \frac{\partial}{\partial y'} = \frac{\partial}{\partial x'} + 2 \frac{\partial}{\partial y'}.$$

So the PDE is transformed into

$$5u_{x'} + 3u = e^{-\frac{x'}{5} + \frac{3y'}{5}}.$$

Consider  $y'$  as a parameter, this equation can be viewed as a first-order inhomogeneous ODE with the independent variable  $x'$ . Let  $u = Ae^{-\frac{x'}{5}}$  be a particular solution, then we have

$$5u_{x'} + 3u = 5 \left( -\frac{A}{5} e^{-\frac{x'}{5}} \right) + 3Ae^{-\frac{x'}{5}} = 2Ae^{-\frac{x'}{5}} = e^{-\frac{x'}{5} + \frac{3y'}{5}}.$$

The coefficient  $A$  is determined as

$$A = \frac{1}{2} e^{\frac{3y'}{5}}.$$

Thus, the particular solution is

$$u(x', y') = \frac{1}{2} e^{-\frac{x'}{5} + \frac{3y'}{5}}.$$

The general solution to the homogeneous equation  $5u_{x'} + 3u = 0$  is  $u(x', y') = f(y')e^{-\frac{3x'}{5}}$ . The solution to the inhomogeneous equation is

$$u(x', y') = f(y')e^{-\frac{3x'}{5}} + \frac{1}{2} e^{-\frac{x'}{5} + \frac{3y'}{5}}.$$

Change back to the original coordinates, we have the solution

$$u(x, y) = f(x + 2y)e^{-\frac{3(-2x+y)}{5}} + \frac{1}{2} e^{-\frac{-2x+y}{5} + \frac{3(x+2y)}{5}},$$

which can be rewritten as

$$u(x, y) = f(x + 2y)e^{\frac{3}{5}(2x-y)} + \frac{1}{2} e^{x+y}.$$

(b) The characteristic curves are given by

$$\frac{dy}{dx} = -\frac{y}{x}.$$

This is a separable ODE, which can be solved to obtain the general solution  $xy = C$ . Thus, our change of coordinates (no need to be orthogonal but should be non-degenerate) will be

$$\begin{cases} x' = x, \\ y' = xy. \end{cases}$$

In these coordinates the equation takes the form

$$x'u_{x'} + \frac{y'^2}{x'^2}u = \frac{y'^2}{x'^2}, \quad \text{or} \quad u_{x'} + \frac{y'^2}{x'^3}u = \frac{y'^2}{x'^3}.$$

Using the integrating factor

$$e^{\int \frac{y'^2}{x'^3} dx'} = e^{-\frac{y'^2}{2x'^2}},$$

the above equation can be written as

$$\left( e^{-\frac{y'^2}{2x'^2}} u \right)_{x'} = e^{-\frac{y'^2}{2x'^2}} \frac{y'^2}{x'^3}.$$

Integrating both sides in  $x'$ , we arrive at

$$e^{-\frac{y'^2}{2x'^2}} u = \int e^{-\frac{y'^2}{2x'^2}} \frac{y'^2}{x'^3} dx' = e^{-\frac{y'^2}{2x'^2}} + f(y').$$

Thus, the general solution will be give by

$$u = e^{\frac{y'^2}{2x'^2}} \left[ e^{-\frac{y'^2}{2x'^2}} + f(y') \right] = 1 + e^{\frac{y'^2}{2x'^2}} f(y').$$

Finally, substituting the expressions of  $x'$  and  $y'$  in terms of  $(x, y)$  into the solution, we obtain

$$u(x, y) = 1 + e^{\frac{y^2}{2}} f(xy).$$

One should again check by substitution that this is indeed a solution to the PDE.

**Problem 10 (Ex. 13 on Page 10)** Use the coordinate method to solve the equation

$$u_x + 2u_y + (2x - y)u = 2x^2 + 3xy - 2y^2.$$

[Solution:] Change variables to

$$x' = x + 2y \quad y' = 2x - y,$$

we have

$$x = (x' + 2y')/5, \quad y = (2x' - y')/5,$$

and

$$\frac{\partial}{\partial x} = \frac{\partial}{\partial x'} + 2\frac{\partial}{\partial y'}, \quad \frac{\partial}{\partial y} = 2\frac{\partial}{\partial x'} - \frac{\partial}{\partial y'}.$$

So the PDE is transformed into

$$u_{x'} + \frac{y'}{5}u = \frac{x'y'}{5}.$$

Consider  $y'$  as a parameter, this equation can be viewed as a first-order inhomogeneous ODE with the independent variable  $x'$ . Let  $P(x') = \int_0^{x'} \frac{y'}{5} ds = \frac{x'y'}{5}$ . Multiplying both sides of the above equation by  $e^{P(x')}$  we get

$$\frac{d}{dx'} \left[ e^{\frac{x'y'}{5}} u \right] = \frac{x'y'}{5} e^{\frac{x'y'}{5}}.$$

Thus, after integrating with respect to  $x'$ , we have

$$e^{\frac{x'y'}{5}} u = \left( x' - \frac{5}{y'} \right) e^{\frac{x'y'}{5}} + f(y'),$$

with  $f$  as an arbitrary function of a single variable. So

$$u(x', y') = \left( x' - \frac{5}{y'} \right) + e^{-\frac{x'y'}{5}} f(y').$$

Change back to the original coordinates, we have the solution

$$u(x, y) = \left( x + 2y - \frac{5}{2x - y} \right) + e^{-\frac{(x+2y)(2x-y)}{5}} f(2x - y).$$

**Problem 11** Find the solution to general constant coefficient linear first-order equations

$$au_x + bu_y + cu = g(x, y).$$

[Solution:] Before we proceed, let's have a review on the following theorem from ODE

**Theorem 1.** *If the functions  $p(x)$ ,  $q(x)$  are continuous, then*

$$y' = p(x)y + q(x), \quad (1)$$

*has infinitely many solutions and every solution,  $y(x)$ , can be labeled by  $r \in R$  as follows*

$$y(x) = re^{P(x)} + e^{P(x)} \int e^{-P(x)} q(x) dx, \quad (2)$$

*where we introduced the function  $P(x) = \int p(x) dx$ , any primitive of the function  $p(x)$ .*  $\square$

We can use the characteristic coordinates  $x' = ax + by$  and  $y' = bx - ay$  to reduce the discussing equation into an inhomogeneous ODE ( $G(x', y') = g(x(x', y'), y(x', y'))$  is assumed.)

$$(a^2 + b^2)u_{x'} + cu = G(x', y'), \quad \text{or} \quad u_{x'} = -\frac{c}{a^2 + b^2}u + \frac{G(x', y')}{a^2 + b^2}.$$

Directly using the above theorem, we have

$$P(x') = \int \left( -\frac{c}{a^2 + b^2} \right) dx' = -\frac{c}{a^2 + b^2}x' + r_1.$$

Here  $r_1$  is constant in  $x'$  (depends only on  $y'$ ). So

$$u(x', y') = r(y')e^{-\frac{c}{a^2+b^2}x' + r_1(y')} + e^{-\frac{c}{a^2+b^2}x' + r_1(y')} \int e^{\frac{c}{a^2+b^2}x' - r_1(y')} \frac{G(x', y')}{a^2 + b^2} dx'.$$

It can be simplified into

$$u(x', y') = f(y')e^{-\frac{c}{a^2+b^2}x'} + e^{-\frac{c}{a^2+b^2}x'} \int e^{\frac{c}{a^2+b^2}x'} \frac{G(x', y')}{a^2 + b^2} dx'.$$

Assume that

$$\int e^{\frac{c}{a^2+b^2}x'} \frac{G(x', y')}{a^2 + b^2} dx' = M(y'),$$

where  $M(y')$  is any primitive of the function  $e^{\frac{c}{a^2+b^2}x'} \frac{G(x', y')}{a^2 + b^2}$  with  $x'$  as the only independent variable and  $y'$  as a parameter. The solution is

$$u(x', y') = e^{-\frac{c}{a^2+b^2}x'} (f(y') + M(y')).$$

Replace  $x'$  and  $y'$  by their expressions in terms of  $x$  and  $y$ , we obtain that

$$u(x, y) = e^{-\frac{c}{a^2+b^2}(ax+by)} [f(bx - ay) + M(bx - ay)].$$

$f$  is an arbitrary function of a single variable.

**Problem 12 (Ex. 1 on Page 19)** Carefully derive the equation of a string in a medium in which the resistance is proportional to the velocity. [Solution:] The derivation is almost the

same as the one shown in Example 2 on Pages 5-11 of Handout 2. The only difference is that

equation (10) should be modified into

$$\int_{x_0}^{x_1} a_u(x, t) \rho dx = T(x_1, t) \frac{u_x(x_1, t)}{\sqrt{1 + u_x^2(x_1, t)}} - T(x_0, t) \frac{u_x(x_0, t)}{\sqrt{1 + u_x^2(x_0, t)}} - \int_{x_0}^{x_1} ru_t(x, t) dx.$$

The red part of the above equation is the resistance. Following the same steps as in Example 2, we can finally get the wave equation with resistance as

$$u_{tt} - c^2 u_{xx} + ru_t = 0, \quad r > 0.$$

**Problem 13 (Ex. 6 on Page 19)** Consider heat flow in a long circular cylinder where the temperature depends only on  $t$  and on the distance  $r$  to the axis of the cylinder. Here  $r = \sqrt{x^2 + y^2}$  is the cylindrical coordinate. From the three-dimensional heat equation derive the equation  $u_t = k(u_{rr} + u_r/r)$ . [Solution:] The three-dimensional heat equation is

$$u_t = k \left( \frac{\partial^2 u}{\partial x^2} + \frac{\partial^2 u}{\partial y^2} + \frac{\partial^2 u}{\partial z^2} \right).$$

The temperature depends only on  $t$  and on the distance  $r$  to the axis of the cylinder. That means the temperature is invariant in the  $z$  direction. The above heat equation can be simplified as

$$u_t = k \left( \frac{\partial^2 u}{\partial x^2} + \frac{\partial^2 u}{\partial y^2} \right).$$

Using the chain rule, we have

$$\frac{\partial u}{\partial x} = \frac{\partial u}{\partial r} \frac{\partial r}{\partial x} = \frac{\partial u}{\partial r} \frac{x}{r}$$

and

$$\begin{aligned} \frac{\partial^2 u}{\partial x^2} &= \frac{\partial}{\partial x} \left( \frac{\partial u}{\partial r} \frac{x}{r} \right) = \frac{x}{r} \frac{\partial}{\partial x} \left( \frac{\partial u}{\partial r} \right) + \frac{\partial u}{\partial r} \frac{\partial}{\partial x} \left( \frac{x}{r} \right) \\ &= \frac{x}{r} \frac{\partial}{\partial r} \left( \frac{\partial u}{\partial r} \right) \frac{\partial r}{\partial x} + \frac{\partial u}{\partial r} \frac{r - x \frac{\partial r}{\partial x}}{r^2} \\ &= \frac{x}{r} \frac{\partial}{\partial r} \left( \frac{\partial u}{\partial r} \right) \frac{x}{r} + \frac{\partial u}{\partial r} \frac{r - x \frac{x}{r}}{r^2} \\ &= \frac{x^2}{r^2} \frac{\partial^2 u}{\partial r^2} + \frac{\partial u}{\partial r} \frac{r^2 - x^2}{r^3}. \end{aligned}$$

Similarly,

$$\frac{\partial^2 u}{\partial y^2} = \frac{y^2}{r^2} \frac{\partial^2 u}{\partial r^2} + \frac{\partial u}{\partial r} \frac{r^2 - y^2}{r^3}.$$

Thus,

$$\begin{aligned} u_t &= k \left( \frac{\partial^2 u}{\partial x^2} + \frac{\partial^2 u}{\partial y^2} \right) = k \left( \frac{x^2}{r^2} \frac{\partial^2 u}{\partial r^2} + \frac{\partial u}{\partial r} \frac{r^2 - x^2}{r^3} + \frac{y^2}{r^2} \frac{\partial^2 u}{\partial r^2} + \frac{\partial u}{\partial r} \frac{r^2 - y^2}{r^3} \right) \\ &= k \left( \frac{x^2 + y^2}{r^2} \frac{\partial^2 u}{\partial r^2} + \frac{\partial u}{\partial r} \frac{2r^2 - x^2 - y^2}{r^3} \right) \\ &= k \left( \frac{\partial^2 u}{\partial r^2} + \frac{1}{r} \frac{\partial u}{\partial r} \right). \end{aligned}$$

**Problem 14** Solve the following first order PDE and find where the solution is defined in the  $x - y$  plane.

$$u_x + xyu_y = 0, \quad u(x, -1) = \frac{1}{2}x^2.$$

[Solution:] The characteristic curves are given by  $\frac{dy}{dx} = \frac{xy}{1}$ . This is a separable ODE. Its

solution is  $\ln|y| = \frac{x^2}{2} + C$ , where  $C$  is any given constant. Further we have  $|y| = e^{x^2/2}e^C$  or  $y = \pm e^{x^2/2}e^C$ . If  $D = \pm e^C$  is any given constant, then  $y = De^{x^2/2}$ . The characteristic curves are given by  $ye^{-x^2/2} = D$ . The general solution of the original PDE is  $u(x, y) = f(ye^{-x^2/2})$ . The auxiliary condition says  $u(x, -1) = \frac{1}{2}x^2$ . Substituting  $y = -1$  into the general solution, we have  $\frac{1}{2}x^2 = f(-e^{-x^2/2})$ . We can only determine the explicit form of  $f(z)$  when its independent variable  $z$  is on the half-closed interval  $[-1, 0)$  as  $f(z) = -\ln(-z)$ . Thus,

$$u(x, y) = \begin{cases} -\ln(-ye^{-x^2/2}) = \ln(-y^{-1}e^{x^2/2}) = \ln(-y^{-1}) + x^2/2, & \text{if } -1 \leq ye^{-x^2/2} < 0; \\ f(ye^{-x^2/2}), & \text{otherwise.} \end{cases}$$

Or,

$$u(x, y) = \begin{cases} \ln(-y^{-1}) + x^2/2, & \text{if } -e^{x^2/2} \leq y < 0; \\ f(ye^{-x^2/2}), & \text{otherwise} \end{cases}$$

From the above discussion, we know that the solution is uniquely determined when  $-e^{x^2/2} \leq y < 0$ .

**Problem 15** Solve the following first order PDE

$$x^2u_x + xyu_y = u.$$

[Solution:] The characteristic curves are given by

$$\frac{dy}{dx} = \frac{xy}{x^2} = \frac{y}{x}.$$

This is a separable ODE, which can be solved to obtain the general solution  $y/x = C$ . Thus, our change of coordinates (no need to be orthogonal but should be non-degenerate) will be

$$\begin{cases} x' = x, \\ y' = \frac{y}{x}. \end{cases}$$

Use the chain rule, we have

$$\begin{cases} \frac{\partial u}{\partial x} = \frac{\partial x'}{\partial x} \frac{\partial u}{\partial x'} + \frac{\partial y'}{\partial x} \frac{\partial u}{\partial y'} = 1 \cdot \frac{\partial u}{\partial x'} - \frac{y}{x^2} \frac{\partial u}{\partial y'} = \frac{\partial u}{\partial x'} - \frac{y'}{x'} \frac{\partial u}{\partial y'}, \\ \frac{\partial u}{\partial y} = \frac{\partial x'}{\partial y} \frac{\partial u}{\partial x'} + \frac{\partial y'}{\partial y} \frac{\partial u}{\partial y'} = 0 \cdot \frac{\partial u}{\partial x'} + \frac{1}{x} \frac{\partial u}{\partial y'} = \frac{1}{x'} \frac{\partial u}{\partial y'}. \end{cases}$$

In these coordinates the equation takes the form

$$x'^2 \left( \frac{\partial u}{\partial x'} - \frac{y'}{x'} \frac{\partial u}{\partial y'} \right) + x'^2 y' \cdot \frac{1}{x'} \frac{\partial u}{\partial y'} = u,$$

or

$$u_{x'} - \frac{1}{x'^2} u = 0.$$

Using the integrating factor

$$e^{\int -\frac{1}{x'^2} dx'} = e^{\frac{1}{x'}},$$



the above equation can be written as

$$\left(e^{\frac{1}{x'}}u\right)_{x'} = 0.$$

Integrating both sides in  $x'$ , we arrive at

$$e^{\frac{1}{x'}}u = f(y').$$

Thus, the general solution will be give by

$$u = e^{-\frac{1}{x'}}f(y').$$

Finally, substituting the expressions of  $x'$  and  $y'$  in terms of  $(x, y)$  into the solution, we obtain

$$u(x, y) = e^{-\frac{1}{x}}f\left(\frac{y}{x}\right).$$

One should again check by substitution that this is indeed a solution to the PDE.